
The turbulent kinetic energy production term can be written in Cartesian coordinates as:
%
%
\begin{equation}
Q_k=\sum_{i=1}^{3} \sum_{j=1}^{3} \frac{\partial \vec{V}^{\rm n}_i}{\partial x_j} \left( \eta^\star \left( \frac{\partial \vec{V}^{\rm n}_i}{\partial x_j}
   + \frac{\partial \vec{V}^{\rm n}_j}{\partial x_i} -\frac{2}{3} \delta_{ij} \sum_{k=1}^{3} \frac{\partial \vec{V}^{\rm n}_k}{\partial x_k}\right) -\frac{2}{3} \rho k \delta_{ij}\right)
\end{equation}
%
where the velocity of the neutrals can be expressed in generalized coordinates as:
%
\begin{equation}
\frac{\partial \vec{V}^{\rm n}_i}{\partial x_j}=\sum_{\theta=1}^{3} X_{\theta,j} \frac{\partial \vec{V}^{\rm n}_i}{\partial X_\theta}
\end{equation}
%
Sustitute the latter in the former:
%
\begin{align}
Q_k=&\sum_{i=1}^{3} \sum_{j=1}^{3} \sum_{\vartheta=1}^{3} X_{\vartheta,j} \frac{\partial \vec{V}^{\rm n}_i}{\partial X_\vartheta} \left( \eta^\star \left( \sum_{\theta=1}^{3} X_{\theta,j} \frac{\partial \vec{V}^{\rm n}_i}{\partial X_\theta}
   + \sum_{\theta=1}^{3} X_{\theta,i} \frac{\partial \vec{V}^{\rm n}_j}{\partial X_\theta} 
-\frac{2}{3} \delta_{ij} \sum_{k=1}^{3} \sum_{\theta=1}^{3} X_{\theta,k} \frac{\partial \vec{V}^{\rm n}_k}{\partial X_\theta}\right)
\right. \nonumber \alb\mfd
&\left.
 -\frac{2}{3} \rho k \delta_{ij}\right)
\end{align}
%
%
\begin{align}
Q_k=&\sum_{i=1}^{3} \sum_{j=1}^{3} \sum_{\vartheta=1}^{3} \sum_{\theta=1}^{3} X_{\vartheta,j} \frac{\partial \vec{V}^{\rm n}_i}{\partial X_\vartheta}
  \eta^\star
    \left(  X_{\theta,j} \frac{\partial \vec{V}^{\rm n}_i}{\partial X_\theta}
       + X_{\theta,i} \frac{\partial \vec{V}^{\rm n}_j}{\partial X_\theta} 
-\frac{2}{3} \delta_{ij} \sum_{k=1}^{3}  X_{\theta,k} \frac{\partial \vec{V}^{\rm n}_k}{\partial X_\theta}
    \right)
 \nonumber \alb\mfd
&
 -\sum_{i=1}^{3} \sum_{\vartheta=1}^{3} X_{\vartheta,i} \frac{\partial \vec{V}^{\rm n}_i}{\partial X_\vartheta} \frac{2}{3} \rho k
\end{align}
%
%
\begin{align}
Q_k=&\sum_{i=1}^{3} \sum_{j=1}^{3} \sum_{\vartheta=1}^{3} \sum_{\theta=1}^{3} X_{\vartheta,j} \frac{\partial \vec{V}^{\rm n}_i}{\partial X_\vartheta}
  \eta^\star
    \left(  X_{\theta,j} \frac{\partial \vec{V}^{\rm n}_i}{\partial X_\theta}
       + X_{\theta,i} \frac{\partial \vec{V}^{\rm n}_j}{\partial X_\theta} -\frac{2}{3} \delta_{ij} \sum_{k=1}^{3}  X_{\theta,k} \frac{\partial \vec{V}^{\rm n}_k}{\partial X_\theta}
    \right)\nonumber
\alb\mfd
 &-\sum_{\theta=1}^{3} \sum_{\vartheta=1}^{3} X_{\theta,\vartheta} \frac{\partial \vec{V}^{\rm n}_\vartheta}{\partial X_\theta} \frac{2}{3} \rho k
\end{align}
%
%
\begin{align}
Q_k=& \sum_{\vartheta=1}^{3} \sum_{\theta=1}^{3}
  \left[
    \sum_{i=1}^{3} \sum_{j=1}^{3} X_{\vartheta,j} \frac{\partial \vec{V}^{\rm n}_i}{\partial X_\vartheta}
    \eta^\star
    \left(  X_{\theta,j} \frac{\partial \vec{V}^{\rm n}_i}{\partial X_\theta}
       + X_{\theta,i} \frac{\partial \vec{V}^{\rm n}_j}{\partial X_\theta} -\frac{2}{3} \delta_{ij} \sum_{k=1}^{3}  X_{\theta,k} \frac{\partial \vec{V}^{\rm n}_k}{\partial X_\theta}
    \right)
\right.\nonumber\alb\mfd
&\left.
    -\frac{2}{3} \rho k X_{\theta,\vartheta} \frac{\partial \vec{V}^{\rm n}_\vartheta}{\partial X_\theta}
  \right]
\end{align}
%

















%
\begin{align}
Q_k= &\sum_{\vartheta=1}^{3} \sum_{\theta=1}^{3}
  \left[
    \sum_{i=1}^{3} \sum_{j=1}^{3} \sum_{m=1}^{3} \sum_{n=1}^{3}
    \eta^\star X_{\theta,n} X_{\vartheta,m} \frac{\partial \vec{V}^{\rm n}_i}{\partial X_\theta} \frac{\partial \vec{V}^{\rm n}_j}{\partial X_\vartheta}
    \left(
     \delta_{ij} \delta_{mn} +\delta_{mi} \delta_{nj} - \frac{2}{3} \delta_{mj} \delta_{ni}
    \right)
\right.\nonumber\alb\mfd
&\left.
    -\frac{2}{3} \rho k X_{\theta,\vartheta} \frac{\partial \vec{V}^{\rm n}_\vartheta}{\partial X_\theta}
  \right]
\end{align}
%
we can express $\beta$ as:
%
%
\begin{equation}
  \beta_{\theta, \vartheta}^{ij}
  =\sum_{m=1}^3 \sum_{n=1}^3 \frac{1}{J}  X_{\vartheta,m} X_{\theta,n}
    \left(
      \delta_{mn}\delta_{ij}+\delta_{im}\delta_{jn}-\frac{2}{3} \delta_{in}\delta_{jm}
    \right)
\end{equation}
%
hence resulting in:
%
\begin{equation}
Q_k=\sum_{\theta=1}^{3} \sum_{\vartheta=1}^{3}
\left( -\frac{2}{3}  \rho k X_{\theta,\vartheta} \frac{\partial \vec{V}^{\rm n}_\vartheta}{\partial X_\theta}
+ \sum_{i=1}^{3} \sum_{j=1}^{3} \eta^\star
 J \beta_{\theta,\vartheta}^{i,j} \frac{\partial \vec{V}^{\rm n}_i}{\partial X_\theta} \frac{\partial \vec{V}^{\rm n}_j}{\partial X_\vartheta}\right)
\end{equation}
%

